theories/simplang/simple_inv/adequacy.v
@@ -1,0 +1,39 @@
+From iris.algebra.lib Require Import gset_bij.
+From iris.base_logic.lib Require Import gset_bij.
+
+From simuliris.logic Require Import satisfiable.
+From simuliris.simulation Require Import slsls global_sim.
+From simuliris.simplang Require Import proofmode tactics.
+From simuliris.simplang Require Import gen_adequacy.
+From simuliris.simplang.simple_inv Require Import inv refl.
+
+Class simpleGpreS Σ := {
+  sbij_pre_heapG :> sheapGpreS Σ;
+  sbij_pre_bijG :> gset_bijG Σ block block;
+}.
+Definition simpleΣ := #[sheapΣ; gset_bijΣ block block].
+
+Global Instance subG_sbijΣ Σ :
+  subG simpleΣ Σ → simpleGpreS Σ.
+Proof. solve_inG. Qed.
+
+Lemma adequacy `{!simpleGpreS Σ} p_t p_s :
+  isat (∀ `(simpleGS Σ), prog_rel p_t p_s) →
+  beh_rel p_t p_s.
+Proof.
+  intros Hprog. apply simplang_adequacy.
+  eapply sat_bupd, sat_mono, Hprog. clear Hprog.
+  iIntros "Hprog_rel".
+  iMod (gset_bij_own_alloc (A:=block) (B:=block) ∅) as (γbij) "[Hbij _]".
+  { apply: gset_bijective_empty. }
+  iIntros "!>" (?).
+  iExists simple_inv, heapbij.loc_rel.
+  set HsimpleGS := SimpleGS Σ (HeapBijG _ _ _ γbij).
+  iSpecialize ("Hprog_rel" $! HsimpleGS).
+  iFrame "Hprog_rel".
+  iSplitL "Hbij".
+  { rewrite /sheap_inv /=. iExists ∅. iFrame.
+    iApply big_sepS_empty. done. }
+  iSplitR; first done.
+  iIntros (??) "$".
+Qed.
